Game/Levels/Lemmas/Partition.lean
@@ -2,6 +2,8 @@ import Mathlib.Order.SetNotation
 import Mathlib.Init.Logic
 import Mathlib.Init.Set
 import Mathlib.Data.Set.Basic
+import Mathlib.Data.SetLike.Basic
+import Mathlib.Tactic
 
 
 /-- A collection `c : Set (Set α)` of sets is a partition of `α` into pairwise
@@ -14,9 +16,10 @@ def IsPartition' (c : Set (Set α)) := ∅ ∉ c ∧ ( ⋃₀ c = Set.univ) ∧ 
 
 
 namespace Setoid
-variable {α :Type*} [inst: Setoid α]
+variable {α :Type*} [inst: Setoid α] {x : α}
 
 abbrev equivclass (x : α):  Set α := {y | x ≈ y}
+
 
 lemma mem_selfequivclass (x : α) : x ∈ Setoid.equivclass x  := by
    rewrite [Set.mem_setOf_eq]
@@ -49,7 +52,121 @@ lemma equivclass_nonempty (x : α) : Setoid.equivclass x ≠ ∅ := by
   intro h
   apply Set.not_mem_empty x
   rw [<-h, Set.mem_setOf_eq]
+
+
+
+
+variable (α) in
+abbrev equivclasses [Setoid α] := {c : Set α // ∃ x, c =  Setoid.equivclass x }
+
+
+variable (α) in
+abbrev Equivclass [Setoid α] := {c : Set α // ∃ x, c =  {y | x ≈ y}}
+
+
+instance equivclass_setlike : SetLike (Equivclass α) α where
+  coe s := s.1
+  coe_injective' _ _ h := Subtype.ext h
+
+
+abbrev quot: α → Equivclass α := fun x => ⟨{y | x ≈ y}, ⟨x,rfl⟩⟩
+
+
+
+--scoped notation3 "[[" x "]]" => (Setoid.quot x)
+
+--variable (x : α)
+--#check Setoid.quot x
+
+lemma mem_quot (x : α) : x ∈ (Setoid.quot x : Equivclass α)  := by
+  --unfold Setoid.quot
   exact Setoid.refl _
+
+
+lemma mem_quot_iff_equiv (x : α): y ∈ Setoid.quot x ↔ x ≈ y := by
+  rfl
+
+
+lemma mem_quot_self (x : α): x ∈ Setoid.quot x := by
+  exact Setoid.refl x
+
+
+lemma exist_quot (c : Equivclass α) : ∃ x, c = Setoid.quot x  := by
+  obtain ⟨c, x, hx⟩ := c
+  use x
+  unfold quot
+  simp only [hx]
+
+
+
+/--
+The equivalence relation `≈` is symmetric.
+-/
+lemma symm_iff {x y : α}: x ≈ y ↔ y ≈ x := ⟨Setoid.symm, Setoid.symm⟩
+
+
+lemma equiv_iff_of_equiv {x y z : α} (H : x ≈ y) : x ≈ z ↔ y ≈ z := by
+  constructor
+  intro H2
+  exact Setoid.trans (Setoid.symm H) H2
+  intro H2
+  exact Setoid.trans H H2
+
+lemma mem_equivclass_of_equiv {c : Setoid.Equivclass α}  (H : x ∈ c) :  x ≈ y  ↔  y ∈ c  := by
+  obtain ⟨z,hz⟩:= exist_quot c
+  rw [hz] at H
+  rw [hz]
+  rw [mem_quot_iff_equiv] at H
+  rw [mem_quot_iff_equiv]
+  replace H := Setoid.symm H
+  exact Setoid.equiv_iff_of_equiv H
+
+
+
+lemma quot_eq_iff_equiv {x y: α} : Setoid.quot x = Setoid.quot y ↔ x ≈ y := by
+  constructor
+  intro H
+  have H2:= Setoid.mem_quot_self y
+  rw [<-H] at H2
+  rw [Setoid.mem_quot_iff_equiv] at H2
+  exact H2
+  intro H
+  rw [SetLike.ext_iff]
+  intro z
+  repeat rw [Setoid.mem_quot_iff_equiv]
+  exact Setoid.equiv_iff_of_equiv H
+
+lemma mem_equivclass_iff_eq_quot {x : α} {c : Equivclass α}  : x ∈ c ↔ c = Setoid.quot x:= by
+  obtain ⟨y, hy⟩ := exist_quot c
+  rw [hy]
+  rw [Setoid.mem_quot_iff_equiv]
+  symm
+  exact Setoid.quot_eq_iff_equiv
+
+
+lemma equivclass_nonempty' (c : Equivclass α) : c.1.Nonempty := by
+  obtain ⟨z, hz⟩ := exist_quot c
+  rw [hz]
+  use z
+  simp only [Set.mem_setOf_eq, refl]
+
+
+noncomputable abbrev Equivclass.unquot : Equivclass α → α :=  fun c => (Setoid.equivclass_nonempty' c).some
+
+lemma Equivclass.unquot_mem {c : Equivclass α} : c.unquot ∈ c := by
+  exact Set.Nonempty.some_mem _
+
+@[simp]
+lemma Equivclass.quot_unquot_eq {c : Equivclass α}: Setoid.quot c.unquot = c := by
+  symm
+  rw [<-Setoid.mem_equivclass_iff_eq_quot]
+  exact c.unquot_mem
+
+
+lemma unquot_quot_equiv : x ≈ (Setoid.quot x).unquot := by
+  rw [<-Setoid.quot_eq_iff_equiv]
+  rw [Equivclass.quot_unquot_eq]
+
 
 
 end Setoid
