Game/Levels/EquivalenceRelation/L06.2_memEquivClass_of_equiv.lean
@@ -1,0 +1,22 @@
+import Game.Metadata
+import Game.Generator.Basic
+-- import Mathlib
+
+World "EquivalenceRelation"
+
+Level 1
+
+
+variable {α :Type*} [inst: Setoid α]
+
+Statement (c : Setoid.equivclasses α)  (h1 : x ∈ c.1)  (h2 : x ≈ y ) : y ∈ c.1  := by
+  obtain ⟨c, z,hz⟩:= c
+  simp only [hz] at *
+  rw [Setoid.mem_equivclass_iff_equiv] at *
+  exact Setoid.trans h1 h2
+
+
+
+
+OnlyTactic rewrite rfl
+OnlyTheorem Set.mem_setOf_eq
