Game/Levels/EquivalenceRelation/L06.2_memsameEquivClass.lean
@@ -1,0 +1,24 @@
+import Game.Metadata
+import Game.Generator.Basic
+-- import Mathlib
+
+World "EquivalenceRelation"
+
+Level 1
+
+
+variable {α :Type*} [inst: Setoid α]
+
+
+Statement (c : Setoid.equivclasses α): x ∈ c.1 ∧ y ∈ c.1  → x ≈ y := by
+  obtain ⟨c, z,hz⟩:= c
+  simp only [hz]
+  rintro ⟨hx,hy⟩
+  rw [Setoid.mem_equivclass_iff_equiv] at *
+  exact Setoid.trans (Setoid.symm hx) hy
+
+
+
+
+OnlyTactic rewrite rfl
+OnlyTheorem Set.mem_setOf_eq
