Game/Levels/EquivalenceRelation/L06.3_EquivClasseq_of_mem.lean
@@ -1,0 +1,23 @@
+import Game.Metadata
+import Game.Generator.Basic
+-- import Mathlib
+
+World "EquivalenceRelation"
+
+Level 1
+
+
+variable {α :Type*} [inst: Setoid α]
+
+
+Statement  (x : α) (c : Setoid.equivclasses α)  (H : x ∈ c.1) : Setoid.equivclass x = c.1:= by
+  ext z
+  rw [Setoid.mem_equivclass_iff_equiv]
+  constructor
+  intro H2
+  exact Setoid.mem_equivclass_of_equiv H H2
+  intro H2
+  exact Setoid.equiv_of_mem_sameclass H H2
+
+OnlyTactic rewrite rfl
+OnlyTheorem Set.mem_setOf_eq
